GCCoordinationSystem draft

Splinter/GCLayer/GCCoordinationSystem.i.dfy
@@ -2,8 +2,8 @@
 // SPDX-License-Identifier: BSD-2-Clause
 
 include "../CoordinationLayer/CoordinationSystem.i.dfy"
-include "CrashTolerantReprJournal.i.dfy"
-include "CrashTolerantReprMap.i.dfy"
+include "GCCrashTolerantJournal.i.dfy"
+include "GCCrashTolerantMap.i.dfy"
 
 // TODO(jonh,robj): This file consists largely of copy-pastage from CoordinationSystem.
 // Figure out how to refactor; maybe create subpredicates in CoordinationSystem to reuse here?
@@ -11,18 +11,15 @@ include "CrashTolerantReprMap.i.dfy"
 // Or maybe it'll get interesting because we're going to begin talking about framing finally.
 
 module GCCoordinationSystem {
-  // import opened Options
-  // import opened MapRemove_s
+  import opened MapRemove_s
   import opened CrashTolerantMapSpecMod
-  // import opened StampedMod
-  // import opened MsgHistoryMod
-  // import opened KeyType
-  // import opened ValueMessage
-  // import opened TotalKMMapMod
+  import opened MsgHistoryMod
+  import opened ValueMessage
+  import opened TotalKMMapMod
   import opened LSNMod
-  import opened CrashTolerantReprJournal
-  import opened CrashTolerantReprMap
-  // import CoordinationSystem
+  import opened GCCrashTolerantJournal
+  import opened GCCrashTolerantMap
+  import CoordinationSystem
 
   import Async = CrashTolerantMapSpecMod.uiopifc.async
   type UIOp = CrashTolerantMapSpecMod.uiopifc.UIOp
@@ -40,8 +37,8 @@ module GCCoordinationSystem {
   }
 
   datatype Variables = Variables(
-    journal: CrashTolerantReprJournal.Variables,
-    mapp: CrashTolerantReprMap.Variables,
+    journal: GCCrashTolerantJournal.Variables,
+    mapp: GCCrashTolerantMap.Variables,
     ephemeral: Ephemeral
   )
   {
@@ -56,20 +53,20 @@ module GCCoordinationSystem {
 
     predicate Init()
     {
-      && CrashTolerantReprJournal.Init(journal)
-      && CrashTolerantReprMap.Init(mapp)
+      && GCCrashTolerantJournal.Init(journal)
+      && GCCrashTolerantMap.Init(mapp)
       && ephemeral.Unknown?
     }
   }
 
-  function SimpleJournalLabel(clbl: CrashTolerantJournal.TransitionLabel) : CrashTolerantReprJournal.TransitionLabel
+  function SimpleJournalLabel(clbl: CrashTolerantJournal.TransitionLabel) : GCCrashTolerantJournal.TransitionLabel
   {
-    CrashTolerantReprJournal.TransitionLabel([], {}, clbl)
+    GCCrashTolerantJournal.TransitionLabel([], {}, clbl)
   }
 
-  function SimpleMapLabel(clbl: CrashTolerantMap.TransitionLabel) : CrashTolerantReprMap.TransitionLabel
+  function SimpleMapLabel(clbl: CrashTolerantMap.TransitionLabel) : GCCrashTolerantMap.TransitionLabel
   {
-    CrashTolerantReprMap.TransitionLabel([], {}, clbl)
+    GCCrashTolerantMap.TransitionLabel([], {}, clbl)
   }
 
   predicate LoadEphemeralFromPersistent(v: Variables, v': Variables, uiop : UIOp)
@@ -78,15 +75,255 @@ module GCCoordinationSystem {
     && uiop.NoopOp?
     && v'.ephemeral.Known?
     // todo(tony): allocs and freed are now constrained in two places, by SimpleJournalLabel(), and journal.LoadEphemeralFromPersistent. Danger.
-    && CrashTolerantReprJournal.Next(v.journal, v'.journal, SimpleJournalLabel(CrashTolerantJournal.LoadEphemeralFromPersistentLabel()))
-    && CrashTolerantReprMap.Next(v.mapadt, v'.mapadt, SimpleMapLabel(CrashTolerantMap.LoadEphemeralFromPersistentLabel(v'.ephemeral.mapLsn)))
+    && GCCrashTolerantJournal.Next(v.journal, v'.journal, SimpleJournalLabel(CrashTolerantJournal.LoadEphemeralFromPersistentLabel()))
+    && GCCrashTolerantMap.Next(v.mapp, v'.mapp, SimpleMapLabel(CrashTolerantMap.LoadEphemeralFromPersistentLabel(v'.ephemeral.mapLsn)))
     && v'.ephemeral.progress == Async.InitEphemeralState()
     && v'.ephemeral.syncReqs == map[]
     // and thus all fields of v' are constrained.
   }
 
-  
+  // Move some journal state into the map to make it (closer to) fresh
+  predicate Recover(v: Variables, v': Variables, uiop : UIOp, records:MsgHistory)
+  {
+    && uiop.NoopOp?
+    && v.WF()
+    && v.ephemeral.Known?
+    && v'.WF()
+    && v'.ephemeral.Known?
 
+    && records.WF()
 
+    // NB that Recover can interleave with mapadt steps (the Betree
+    // reorganizing its state, possibly flushing stuff out to disk).
+    && GCCrashTolerantJournal.Next(v.journal, v'.journal, SimpleJournalLabel(CrashTolerantJournal.ReadForRecoveryLabel(records)))
+    && GCCrashTolerantMap.Next(v.mapp, v'.mapp, SimpleMapLabel(CrashTolerantMap.PutRecordsLabel(records)))
 
+    && v'.ephemeral == v.ephemeral.(mapLsn := records.seqEnd) // all else defined via predicates above
+  }
+
+  predicate AcceptRequest(v: Variables, v': Variables, uiop : UIOp)
+  {
+    && v.ephemeral.Known?
+    && uiop.OperateOp?
+    && uiop.baseOp.RequestOp?
+    && uiop.baseOp.req !in v.ephemeral.progress.requests
+    && v' == v.(ephemeral := v.ephemeral.(progress := v.ephemeral.progress.(
+        requests := v.ephemeral.progress.requests + {uiop.baseOp.req})))
+  }
+
+  predicate Query(v: Variables, v': Variables, uiop : UIOp)
+  {
+    && v.WF()
+    && v'.WF()
+    && v.ephemeral.Known?
+    && v'.ephemeral.Known?
+    && uiop.OperateOp?
+    && uiop.baseOp.ExecuteOp?
+    && uiop.baseOp.req.input.GetInput? // ensures that the uiop translates to a Get op
+    && uiop.baseOp.reply.output.GetOutput?
+    && uiop.baseOp.req in v.ephemeral.progress.requests
+    && uiop.baseOp.reply.id == uiop.baseOp.req.id
+
+    && uiop.baseOp.req in v.ephemeral.progress.requests
+    && uiop.baseOp.reply !in v.ephemeral.progress.replies
+    && var key := uiop.baseOp.req.input.key;
+    && var value := uiop.baseOp.reply.output.value;
+    && assert AnyKey(key);
+
+    // Journal confirms that the map is up-to-date (but otherwise doesn't do anything).
+    && GCCrashTolerantJournal.Next(v.journal, v'.journal, SimpleJournalLabel(CrashTolerantJournal.QueryEndLsnLabel(v.ephemeral.mapLsn)))
+    // Map handles the query
+    && GCCrashTolerantMap.Next(v.mapp, v'.mapp, SimpleMapLabel(CrashTolerantMap.QueryLabel(v.ephemeral.mapLsn, key, value)))
+
+    && v'.ephemeral == v.ephemeral.(progress := v.ephemeral.progress.(
+          requests := v.ephemeral.progress.requests - {uiop.baseOp.req},
+          replies := v.ephemeral.progress.replies + {uiop.baseOp.reply}
+      ))
+  }
+
+  predicate Put(v: Variables, v': Variables, uiop : UIOp)
+  {
+    // At this layer we allow puts to run ahead, and then just let Queries be
+    // delayed until Recover catches up the mapadt.
+    // We expect the real implementation to maintain the invariant that, after
+    // recovery, the map stays "fresh" with the puts in the journal rather than
+    // checking that property at each query.
+    && v.WF()
+    && v'.WF()
+    && v.ephemeral.Known?
+    && v'.ephemeral.Known?
+
+    && uiop.OperateOp?
+    && uiop.baseOp.ExecuteOp?
+    && uiop.baseOp.req.input.PutInput? // ensures that the uiop translates to a put op
+    && uiop.baseOp.reply.output.PutOutput?
+    && uiop.baseOp.req in v.ephemeral.progress.requests
+    && uiop.baseOp.reply.id == uiop.baseOp.req.id
+    && uiop.baseOp.reply !in v.ephemeral.progress.replies
+
+    && var key := uiop.baseOp.req.input.key;
+    && var val := uiop.baseOp.req.input.value;
+
+    && var singleton := MsgHistoryMod.SingletonAt(v.ephemeral.mapLsn, KeyedMessage(key, Define(val)));
+
+    && v.WF()
+    && GCCrashTolerantJournal.Next(v.journal, v'.journal, SimpleJournalLabel(CrashTolerantJournal.PutLabel(singleton)))
+    && GCCrashTolerantMap.Next(v.mapp, v'.mapp, SimpleMapLabel(CrashTolerantMap.PutRecordsLabel(singleton)))
+
+    && v'.ephemeral == v.ephemeral.(
+          mapLsn := v.ephemeral.mapLsn + 1,
+          progress := v.ephemeral.progress.(
+            requests := v.ephemeral.progress.requests - {uiop.baseOp.req},
+            replies := v.ephemeral.progress.replies + {uiop.baseOp.reply}
+          // syncReqs UNCHANGED
+          )
+      )
+  }
+
+  predicate DeliverReply(v: Variables, v': Variables, uiop : UIOp)
+  {
+    && v.ephemeral.Known?
+    && uiop.OperateOp?
+    && uiop.baseOp.ReplyOp?
+    && uiop.baseOp.reply in v.ephemeral.progress.replies
+    && v' == v.(ephemeral := v.ephemeral.(progress := v.ephemeral.progress.(
+        replies := v.ephemeral.progress.replies - {uiop.baseOp.reply})))
+  }
+
+  // Journal Internal steps (writing stuff out to disk, for example)
+  // and Betree Internal steps (writing stuff to disk, flushing and compacting,
+  // which create new blocks in cache and rearrange the indirection table)
+  // all look like stutters at this layer.
+
+  predicate JournalInternal(v: Variables, v': Variables, uiop : UIOp)
+  {
+    && v.ephemeral.Known?
+    && v'.ephemeral.Known?
+    && uiop.NoopOp?
+    // TODO(tony): is having an 'exists' here a good idea?
+    // journal internal step that maybe does GC
+    // lbl.alloc and freed are constrained by GCCrashTolerantJournal.Next
+    && (exists lbl: GCCrashTolerantJournal.TransitionLabel ::
+        && lbl.base.InternalLabel?
+        && GCCrashTolerantJournal.Next(v.journal, v'.journal, lbl)
+        && v' == v.(journal := v'.journal)  // predicate update above
+    )
+  }
+
+  predicate MapInternal(v: Variables, v': Variables, uiop : UIOp)
+  {
+    && v.ephemeral.Known?
+    && v'.ephemeral.Known?
+    && uiop.NoopOp?
+    // TODO(tony): is having an 'exists' here a good idea?
+    // Map internal step that maybe does GC
+    // lbl.alloc and freed are constrained by GCCrashTolerantMap.Next
+    && (exists lbl: GCCrashTolerantMap.TransitionLabel ::
+        && lbl.base.InternalLabel?
+        && GCCrashTolerantMap.Next(v.mapp, v'.mapp, lbl)
+        && v' == v.(mapp := v'.mapp)  // predicate update above
+    )
+  }
+
+  predicate ReqSync(v: Variables, v': Variables, uiop : UIOp)
+  {
+    && v.WF()
+    && v'.WF()
+    && v.ephemeral.Known?
+    && v'.ephemeral.Known?
+    && uiop.ReqSyncOp?
+    && uiop.syncReqId !in v.ephemeral.syncReqs
+
+    // TODO(robj): cleanup: delete this predicate; it's probably totally unecessary.
+    // Need to record the current LSN, which is generally the current map state. But we
+    // also need to confirm that the journal hasn't gone ahead, since sync is relative to
+    // writes (which have affected the journal).
+    && GCCrashTolerantJournal.Next(v.journal, v'.journal, SimpleJournalLabel(CrashTolerantJournal.QueryEndLsnLabel(v.ephemeral.mapLsn)))
+
+    && v'.mapp == v.mapp
+
+    // NB that the label for a sync in the table is the LSN AFTER the last write
+    && v'.ephemeral == v.ephemeral.(
+        syncReqs := v.ephemeral.syncReqs[uiop.syncReqId := v.ephemeral.mapLsn]
+      )
+  }
+
+  predicate ReplySync(v: Variables, v': Variables, uiop : UIOp)
+  {
+    && v.WF()
+    && v.ephemeral.Known?
+    && uiop.ReplySyncOp?
+    && uiop.syncReqId in v.ephemeral.syncReqs
+    && GCCrashTolerantJournal.Next(v.journal, v'.journal, SimpleJournalLabel(CrashTolerantJournal.QueryLsnPersistenceLabel(v.ephemeral.syncReqs[uiop.syncReqId])))
+    && v' == v.(ephemeral := v.ephemeral.(
+        syncReqs := MapRemove1(v.ephemeral.syncReqs, uiop.syncReqId)
+      ))
+  }
+
+  // This step models issuing the superblock write
+  predicate CommitStart(v: Variables, v': Variables, uiop : UIOp, newBoundaryLsn: LSN)
+  {
+    && uiop.NoopOp?
+    && v.WF()
+    && v.ephemeral.Known?
+
+    && GCCrashTolerantJournal.Next(v.journal, v'.journal, SimpleJournalLabel(CrashTolerantJournal.CommitStartLabel(newBoundaryLsn, v.ephemeral.mapLsn)))
+    && GCCrashTolerantMap.Next(v.mapp, v'.mapp, SimpleMapLabel(CrashTolerantMap.CommitStartLabel(newBoundaryLsn)))
+
+    && v'.ephemeral == v.ephemeral  // UNCHANGED
+  }
+
+  // This step models learning that the outstanding superblock write has completed.
+  predicate CommitComplete(v: Variables, v': Variables, uiop : UIOp)
+  {
+    && v.WF()
+    && v'.WF()
+    && uiop.SyncOp?
+    && v.ephemeral.Known? // provable from invariant
+
+    && GCCrashTolerantJournal.Next(v.journal, v'.journal, SimpleJournalLabel(CrashTolerantJournal.CommitCompleteLabel(v.ephemeral.mapLsn)))
+    && GCCrashTolerantMap.Next(v.mapp, v'.mapp, SimpleMapLabel(CrashTolerantMap.CommitCompleteLabel()))
+
+    && v'.ephemeral == v.ephemeral  // UNCHANGED
+  }
+
+  predicate Crash(v: Variables, v': Variables, uiop : UIOp)
+  {
+    && v.WF()
+    && v'.WF()
+    && uiop.CrashOp?
+
+    && GCCrashTolerantJournal.Next(v.journal, v'.journal, SimpleJournalLabel(CrashTolerantJournal.CrashLabel()))
+    && GCCrashTolerantMap.Next(v.mapp, v'.mapp, SimpleMapLabel(CrashTolerantMap.CrashLabel()))
+
+    && v'.ephemeral.Unknown?
+  }
+
+  predicate Init(v: Variables) {
+    v.Init()
+  }
+
+  type Step = CoordinationSystem.Step // laaaazy
+
+  predicate NextStep(v: Variables, v': Variables, uiop : UIOp, step: Step) {
+    match step {
+      case LoadEphemeralFromPersistentStep() => LoadEphemeralFromPersistent(v, v', uiop)
+      case RecoverStep(puts) => Recover(v, v', uiop, puts)
+      case AcceptRequestStep() => AcceptRequest(v, v', uiop)
+      case QueryStep() => Query(v, v', uiop)
+      case PutStep() => Put(v, v', uiop)
+      case DeliverReplyStep() => DeliverReply(v, v', uiop)
+      case JournalInternalStep() => JournalInternal(v, v', uiop)
+      case MapInternalStep() => MapInternal(v, v', uiop)
+      case ReqSyncStep() => ReqSync(v, v', uiop)
+      case ReplySyncStep() => ReplySync(v, v', uiop)
+      case CommitStartStep(newBoundaryLsn) => CommitStart(v, v', uiop, newBoundaryLsn)
+      case CommitCompleteStep() => CommitComplete(v, v', uiop)
+      case CrashStep() => Crash(v, v', uiop)
+    }
+  }
+
+  predicate Next(v: Variables, v': Variables, uiop: UIOp) {
+    exists step :: NextStep(v, v', uiop, step)
+  }
 }
